messageInvariantPrototypes/twoPhaseCommit/decentralized/messageInvariants.dfy
@@ -29,20 +29,33 @@ ghost predicate VoteMsgAgreeWithVoter(c: Constants, v: Variables)
 
 // DecideMsgs should reflect the decision of the leader
 // Note that this hinges on fact that leader does not equivocate
-ghost predicate DecisionMsgsAgreeWithLeader(c: Constants, v: Variables)
+ghost predicate DecisionMsgsAgreeWithLeader1(c: Constants, v: Variables)
   requires v.WF(c)
 {
   forall msg | msg in v.network.sentMsgs && msg.DecideMsg? 
-  :: v.GetCoordinator(c).decision.WOSome? && msg.decision == v.GetCoordinator(c).decision.value
+  :: v.GetCoordinator(c).decision.WOSome?
+}
+
+ghost predicate DecisionMsgsAgreeWithLeader2(c: Constants, v: Variables)
+  requires v.WF(c)
+{
+  forall msg | msg in v.network.sentMsgs && msg.DecideMsg? && v.GetCoordinator(c).decision.WOSome?
+  :: msg.decision == v.GetCoordinator(c).decision.value
 }
 
 // If a participant has decided, then there must be a corresponding DecideMsg
-ghost predicate ParticipantsDecisionImpliesDecideMsg(c: Constants, v: Variables) 
+ghost predicate ParticipantsDecisionImpliesDecideMsg1(c: Constants, v: Variables) 
   requires v.WF(c)
 {
-  forall i | c.ValidParticipantId(i) && PartipantHasDecided(c, v, i) :: 
-    && (ParticipantDecidedCommit(c, v, i) ==> DecideMsg(Commit) in v.network.sentMsgs)
-    && (ParticipantDecidedAbort(c, v, i) ==> DecideMsg(Abort) in v.network.sentMsgs)
+  forall i | c.ValidParticipantId(i) && PartipantHasDecided(c, v, i) 
+  :: (ParticipantDecidedCommit(c, v, i) ==> DecideMsg(Commit) in v.network.sentMsgs)
+}
+
+ghost predicate ParticipantsDecisionImpliesDecideMsg2(c: Constants, v: Variables) 
+  requires v.WF(c)
+{
+  forall i | c.ValidParticipantId(i) && PartipantHasDecided(c, v, i) 
+  :: (ParticipantDecidedAbort(c, v, i) ==> DecideMsg(Abort) in v.network.sentMsgs)
 }
 
 ghost predicate MessageInv(c: Constants, v: Variables)
@@ -50,8 +63,10 @@ ghost predicate MessageInv(c: Constants, v: Variables)
   && v.WF(c)
   && VoteMsgValidSrc(c, v)
   && VoteMsgAgreeWithVoter(c, v)
-  && DecisionMsgsAgreeWithLeader(c, v)
-  && ParticipantsDecisionImpliesDecideMsg(c, v)
+  && DecisionMsgsAgreeWithLeader1(c, v)
+  && DecisionMsgsAgreeWithLeader2(c, v)
+  && ParticipantsDecisionImpliesDecideMsg1(c, v)
+  && ParticipantsDecisionImpliesDecideMsg2(c, v)
 }
 
 lemma InitImpliesMessageInv(c: Constants, v: Variables)
