messageInvariantPrototypes/twoPhaseCommit/automate/readme.md
@@ -1,0 +1,4 @@
+# Readme
+
+* Extraneous message invariants:
+  * `SendVoteReqMsgValidity`
